----------------------------------------
Let \[f(x) =
\begin{cases}
x/2 &\quad \text{if } x \text{ is even}, \\
3x+1 &\quad \text{if } x \text{ is odd}.
\end{cases}
\]What is $f(f(f(f(1))))$?
Evaluating each value, $f(1) = 3 \cdot 1 + 1 = 4$; $f(f(1)) = f(4) = 4/2 = 2$; $f(f(f(1))) = f(2) = 2/2 = 1$; and finally $f(f(f(f(1)))) = f(1) = \boxed{4}$.
f(1) = 4 <sep> f(4) = 2 <sep> f(2) = 1 <sep> f(1) = 4
----------------------------------------
Finish extracting cv
----------------------------------------
Let \[f(x) =
\begin{cases}
2x^2 - 3&\text{if } x\le 2, \\
ax + 4 &\text{if } x>2.
\end{cases}
\]Find $a$ if the graph of $y=f(x)$ is continuous (which means the graph can be drawn without lifting your pencil from the paper).
If the graph of $f$ is continuous, then the graphs of the two cases must meet when $x=2,$ which (loosely speaking) is the dividing point between the two cases. Therefore, we must have $2\cdot 2^2 -3 = 2a + 4.$ Solving this equation gives $a = \boxed{\frac{1}{2}}.$
continuous graph <sep> x = 2 <sep> 2 * 2^2 - 3 <sep> 2a + 4 <sep> solving equation
----------------------------------------
Finish extracting cv
----------------------------------------
Simplify $\sqrt[3]{1+8} \cdot \sqrt[3]{1+\sqrt[3]{8}}$.
The first cube root becomes $\sqrt[3]{9}$. $\sqrt[3]{8}=2$, so the second cube root becomes $\sqrt[3]{3}$. Multiplying these gives $\sqrt[3]{27} = \boxed{3}$.
sqrt[3]{9} <sep> sqrt[3]{8} = 2 <sep> sqrt[3]{3} <sep> sqrt[3]{27} = 3
----------------------------------------
Finish extracting cv
----------------------------------------
The points $(9, -5)$ and $(-3, -1)$ are the endpoints of a diameter of a circle. What is the sum of the coordinates of the center of the circle?
The center of the circle is located at the midpoint of any diameter. Thus, the center of the circle is $\left(\frac{9+(-3)}{2}, \frac{(-5)+(-1)}{2}\right) = (3, -3)$. The sum of the coordinates of the center of the circle is therefore $3 + (-3) = \boxed{0}$.
midpoint of diameter <sep> (9 + (-3))/2 <sep> (-5 + (-1))/2 <sep> (3, -3) <sep> sum of coordinates 0
----------------------------------------
Finish extracting cv
----------------------------------------
Let $f(x)=x^3+3$ and $g(x) = 2x^2 + 2x +1$. What is $g(f(-2))$?
We note that $f(-2)=(-2)^3+3=-5$, so $g(f(-2))=g(-5)=2\cdot(-5)^2+2\cdot(-5)+1=41.$ Therefore our answer is $\boxed{41}$.
f(-2) = (-2)^3 + 3 <sep> -5 <sep> g(-5) <sep> 2*(-5)^2 + 2*(-5) + 1
----------------------------------------
Finish extracting cv
----------------------------------------
Three faucets fill a 100-gallon tub in 6 minutes.  How long, in seconds, does it take six faucets to fill a 25-gallon tub?  Assume that all faucets dispense water at the same rate.
Since three faucets can fill a 100-gallon tub in 6 minutes, six can do it twice as fast, i.e. 3 minutes.  Additionally, the tub is a quarter the size and thus it will be filled four times as fast which gives $3/4$ minutes or $\boxed{45}$ seconds.
three faucets 100-gallon 6 minutes <sep> six faucets twice as fast <sep> 3 minutes <sep> quarter the size <sep> four times as fast <sep> 3/4 minutes <sep> 45 seconds
----------------------------------------
Finish extracting cv
----------------------------------------
Berengere and her American foreign-exchange student Emily are at a bakery in Paris that accepts both euros and American dollars. They want to buy a cake, but neither of them has enough money. If the cake costs 6 euros and Emily has an American five-dollar bill, how many euros does Berengere need to contribute to the cost of the cake if 1 euro = 1.25 USD?
The easiest way to solve this problem is to convert everything into euros. Emily's five-dollar bill is equivalent to $5\text{ USD} \times \frac{1\text{ euro}}{1.25\text{ USD}}=4\text{ euros}$. Since the girls need 6 euros between them, Berengere must contribute $6-4=\boxed{2 \text{ euros}}$.
convert to euros <sep> 5 USD to euros <sep> 1 euro = 1.25 USD <sep> 6 - 4
----------------------------------------
Finish extracting cv
----------------------------------------
Consider the given functions: $$\begin{array}{ccc}
f(x) & = & 5x^2 - \frac{1}{x}+ 3\\
g(x) & = & x^2-k
\end{array}$$If $f(2) - g(2) = 2$, what is the value of $k$?
We substitute $f(2) = 5(2)^2 - \frac{1}{2} + 3 = \frac{45}{2}$ and $g(2) = (2)^2 - k = 4 - k$. So $f(2) - g(2) = 2$ gives us $\frac{45}{2} - 4 + k=2$. Solving for $k$, we find $k = \frac{4}{2} - \frac{45}{2} + \frac{8}{2}$ so $\boxed{k = \frac{-33}{2}}$.
f(2) = 5(2)^2 - 1/2 + 3 <sep> g(2) = (2)^2 - k <sep> 45/2 - 4 + k = 2 <sep> solving for k <sep> k = 4/2 - 45/2 + 8/2
----------------------------------------
Finish extracting cv
----------------------------------------
Let \[f(x) =
\begin{cases}
3x^2 + 2&\text{if } x\le 3, \\
ax - 1 &\text{if } x>3.
\end{cases}
\]Find $a$ if the graph of $y=f(x)$ is continuous (which means the graph can be drawn without lifting your pencil from the paper).
If the graph of $f$ is continuous, then the graphs of the two cases must meet when $x=3$, which (loosely speaking) is the dividing point between the two cases.  Therefore, we must have $3(3^2) + 2 = 3a - 1$.  Solving this equation gives $a = \boxed{10}$.
x = 3 <sep> 3(3^2) + 2 <sep> 3a - 1 <sep> continuous graph <sep> dividing point between cases
----------------------------------------
Finish extracting cv
----------------------------------------
The greatest integer function, $\lfloor x\rfloor$, denotes the largest integer less than or equal to $x$. For example, $\lfloor3.5\rfloor=3$, $\lfloor\pi\rfloor=3$ and $\lfloor -\pi\rfloor=-4$. Find the sum of the three smallest positive solutions to $x-\lfloor x\rfloor=\frac1{\lfloor x\rfloor}.$ Express your answer as a mixed number.
We will begin with the smallest possible positive values of $x$.  For positive values of $x$, when $0<x<1$, the right side of our equation is equal to $\frac{1}{0}$, which is undefined. When $1 \le x < 2$  , the right side of our equation is equal to $1$, but $x - \lfloor x \rfloor $ cannot equal $1$.

When $2 \le x<3$, the right side of our equation is equal to $\frac{1}{2}$, so we have $x - \lfloor x \rfloor = \frac{1}{2}$.  This occurs when $x = 2 \frac{1}{2}$.

When $3 \le x<4$, the right side of our equation is equal to $\frac{1}{3}$, so we have $x - \lfloor x \rfloor = \frac{1}{3}$.  This occurs when $x = 3 \frac{1}{3}$.

When $4 \le x<5$, the right side of our equation is equal to $\frac{1}{4}$, so we have $x - \lfloor x \rfloor = \frac{1}{4}$.  This occurs when $x = 4 \frac{1}{4}$.

Then the sum of the three smallest positive solutions to $x$ is $2 \frac{1}{2} +3 \frac{1}{3}+4 \frac{1}{4} = \boxed{10\frac{1}{12}}.$
0 < x < 1 <sep> undefined <sep> 1 ≤ x < 2 <sep> x - ⌊x⌋ ≠ 1 <sep> 2 ≤ x < 3 <sep> 1/2 <sep> x = 2 1/2 <sep> 3 ≤ x < 4 <sep> 1/3 <sep> x = 3 1/3 <sep> 4 ≤ x < 5 <sep> 1/4 <sep> x = 4 1/4 <sep> sum 2 1/2 + 3 1/3 + 4 1/4
----------------------------------------